theories/Weakening.v
@@ -3,6 +3,4 @@ From MetaCoq.PCUIC Require Import PCUICAst.
 Definition isRel t :=
     match t with tRel _ => true | _ => false end.
 
-
-
 Definition eta {A B : Type} (f : A -> B) : f = (fun x => f x) := eq_refl.
